\documentclass{article}
\usepackage{amsmath}
\usepackage{amsfonts}
\usepackage{mathbbol}
\usepackage{mathtools}
\usepackage[letterpaper,top=1in,bottom=1in,left=1in,right=1in]{geometry}
\usepackage{chngcntr}
\usepackage{amssymb}
\usepackage[verbose]{placeins}
\counterwithin*{equation}{section}
\counterwithin*{equation}{subsection}
\renewcommand{\thesubsection}{\thesection.\alph{subsection}}

\DeclarePairedDelimiter{\floor}{\lfloor}{\rfloor}
\DeclarePairedDelimiter{\ceil}{\lceil}{\rceil}

\title{Written Assignment 7}
\author{Daniel Detore\\CS135 B/LF}
\date{April 4, 2024}

\begin{document}
\maketitle
\raggedright

\section{}
\subsection{}
\begin{align*}
    T(1) &= 2T(\floor{\frac{1}{4}}) + \sqrt{1} \\
         &= 2T(0) + 1 \\
         &= 2(1) + 1 \\
    T(1) &= 3
\end{align*}
\begin{align*}
    T(2) &= 2T(\floor{\frac{2}{4}}) + \sqrt{2} \\
         &= 2T(0) + \sqrt{2} \\
    T(2) &= 2 + \sqrt{2}\\
         &\approx 3.41421
\end{align*}

\subsection{}
We need to prove that $T(n) \leq 3\sqrt{n}\log_2 n$ for all $n\geq 2$.\\
Let's check this premise for basis $n=2$:
\begin{align*}
    T(2) &\leq 3\sqrt{2}\log_2(2) \\
    2 + \sqrt{2} &\leq 3\sqrt{2} \\
    2 &\leq 2\sqrt{2} \\
    1 &\leq \sqrt{2} \\
    &\top
\end{align*}
Note the use of (a) in the second equation.\\
Inductive hypothesis: Let $k$ be an integer $\geq 2$. We'll assume that $T(i) \leq 3\sqrt{i}\log_2 i$ for all $2 \leq i\leq k, i\in \mathbb{Z}$.\\
Now we must prove that
\begin{equation*}
    T(k+1) \leq 3\sqrt{k+1}\log_2(k+1).
\end{equation*}
\begin{align*}
    T(k+1) &= 2T(\floor*{\frac{k+1}{4}}) + \sqrt{k+1} & \text{By definition of $T$}\\
           &\leq 2(3\sqrt{\floor*{\frac{k+1}{4}}}\log_2\floor*{\frac{k+1}{4}}) + \sqrt{k+1} & \text{By the inductive hypothesis} \\
           &\leq 2(3\sqrt{\frac{k+1}{4}}\log_2(\frac{k+1}{4})) + \sqrt{k+1} & \floor{x} \leq x \\
           &= 2(\frac{3}{2}\sqrt{k+1}\log_2(\frac{k+1}{4})) + \sqrt{k+1} & \text{By algebra} \\
           &= 3\sqrt{k+1}\log_2(\frac{k+1}{4}) + \sqrt{k+1} \\
           &= 3\sqrt{k+1}(\log_2(k+1) - \log_2(4)) + \sqrt{k+1} \\
           &= 3\sqrt{k+1}(\log_2(k+1) - 2) + \sqrt{k+1} \\
           &= 3\sqrt{k+1}\log_2(k+1) - 6\sqrt{k+1} + \sqrt{k+1} \\
           &= 3\sqrt{k+1}\log_2(k+1) - 5\sqrt{k+1} \\
           &< 3\sqrt{k+1}\log_2(k+1)                                    &\blacksquare
\end{align*}


\end{document}